src/Parsers/StringLike/Core.v
@@ -41,6 +41,6 @@ Definition str_le {CharType} {String : string_like CharType} (s1 s2 : String)
 Infix "≤s" := str_le (at level 70, right associativity).
 
 
-Record StringWithSplitState {CharType} (String : string_like CharType) (split_stateT : Type) :=
+Record StringWithSplitState {CharType} (String : string_like CharType) (split_stateT : String -> Type) :=
   { string_val :> String;
-    state_val : split_stateT }.
+    state_val : split_stateT string_val }.
